proofs/transform/eliminate_algebraic_proofs/eliminate_algebraic_typing.v
@@ -1,0 +1,168 @@
+Require Import Task eliminate_algebraic eliminate_algebraic_context.
+Set Bullet Behavior "Strict Subproofs".
+
+Section Proofs.
+(*TODO: will we need to case on this?*)
+Variable (new_constr_name: funsym -> string).
+Variable keep_muts : mut_adt -> bool.
+
+Variable badnames : list string.
+(*TODO: assume that badnames includes all ids in gamma*)
+
+
+(* Variable (cc_maps: list funsym -> amap funsym funsym). *)
+Variable (noind: typesym -> bool).
+
+(*Let's do delta first*)
+
+
+
+(*Prove context is valid*)
+
+(*Prove for 2 different gamma1 and gamma2 for induction*)
+
+(*Not true: need to ensure anything added to gamma2 not in gamma1*)
+(* Lemma change_context_cons (d: def) (gamma1 gamma2: context):
+  sublist_sig gamma1 gamma2  ->
+  valid_context (d :: gamma1) ->
+  valid_context gamma2 ->
+  valid_context (d :: gamma2).
+Proof.
+  intros Hsub gamma_valid Hval2.
+  pose proof (sub_sig_idents _ _ Hsub) as Hidents.
+  unfold sublist_sig in Hsub.
+  destruct Hsub as [Hsubt [Hsubf Hsubp]].
+  inversion gamma_valid; subst.
+  constructor; auto.
+  - revert H2. apply Forall_impl.
+    intros f. apply wf_funsym_sublist.
+    unfold sig_t in *; simpl.
+    apply sublist_app2; auto. apply sublist_refl.
+  - revert H3. apply Forall_impl.
+    intros p. apply wf_predsym_sublist.
+    unfold sig_t in *; simpl.
+    apply sublist_app2; auto. apply sublist_refl.
+  - intros x [Hinx1 Hinx2]. *)
+
+
+(* Lemma comp_ctx_gamma_valid (g1 g2: context) (g2_sub: sublist g2 g1) (*TODO: this? or just mut?*) 
+  (gamma_valid: valid_context g2):
+  valid_context (concat (map (fun d => comp_ctx_gamma new_constr_name keep_muts badnames
+    noind d g1) g2)).
+Proof.
+  induction g2 as [| d g2 IH]; simpl; [constructor|].
+  assert (Hsub: sublist g2 g1). {
+    intros x Hinx. apply g2_sub. simpl; auto.
+  }
+  inversion gamma_valid; subst.
+  destruct d; simpl; auto.
+  2: {
+    constructor; auto.
+  }
+  unfold comp_ctx_gamma.
+  destruct d *)
+
+
+(* Lemma fold_all_ctx_gamma_valid tsk (Hty: task_typed tsk):
+  valid_context (fold_all_ctx_gamma new_constr_name keep_muts badnames noind tsk).
+Proof.
+  (*Really just need that tsk is valid (I think) - might also need to assume badnames
+    is subset of existing*)
+  assert (gamma_valid: valid_context (task_gamma tsk)). { inversion Hty; subst; auto. }
+  clear Hty.
+  unfold fold_all_ctx_gamma. *)
+
+Lemma tfun_ty_change_sym gamma (f1 f2: funsym) tys tms ty:
+  s_args f1 = s_args f2 ->
+  s_params f1 = s_params f2 ->
+  f_ret f1 = f_ret f2 ->
+  In f2 (sig_f gamma) ->
+  term_has_type gamma (Tfun f1 tys tms) ty ->
+  term_has_type gamma (Tfun f2 tys tms) ty.
+Proof.
+  intros Hargs Hparams Hret Hsig Hty. inversion Hty; subst.
+  rewrite Hret, Hparams. apply T_Fun; auto.
+  - rewrite <- Hret; auto.
+  - rewrite <- Hargs; auto.
+  - rewrite <- Hparams; auto.
+  - rewrite <- Hparams, <- Hargs; auto.
+Qed.
+
+(*Prove that [rewriteT/rewriteF] well typed*)
+Lemma rewrite_typed tsk (*TODO: gamma?*) names t f:
+  (forall ty (Hty: term_has_type 
+    (fold_all_ctx_gamma new_constr_name keep_muts badnames noind tsk) t ty),
+  term_has_type (fold_all_ctx_gamma new_constr_name keep_muts badnames noind tsk)
+    (rewriteT keep_muts new_constr_name badnames 
+      (fold_all_ctx_gamma new_constr_name keep_muts badnames noind tsk)
+      names t) ty) /\
+  (forall av sign (Hf: formula_typed 
+    (fold_all_ctx_gamma new_constr_name keep_muts badnames noind tsk) f),
+    formula_typed (fold_all_ctx_gamma new_constr_name keep_muts badnames noind tsk)
+      (rewriteF keep_muts new_constr_name badnames
+        (fold_all_ctx_gamma new_constr_name keep_muts badnames noind tsk)
+        names av sign f)).
+Proof.
+  revert t f.
+  apply term_formula_ind; auto.
+  - (*Tfun*) intros f1 tys tms IH ty Hty.
+    simpl.
+    destruct (_ && _) eqn : Hb.
+    + apply tfun_ty_change_sym with (f1:=f1); auto.
+      (*Need to prove [sig_f] - TODO: prove sig_f, sig_t, sig_p for new context
+        need for this and wf context - should be very similar to interp*)
+      (*START*)
+
+
+    inversion Hty; subst.
+    simpl.
+    destruct ()
+     apply T_Fun. constructor.
+  
+   simpl. auto.
+
+
+Theorem fold_comp_sound:
+  typed_trans
+  (fold_comp keep_muts new_constr_name badnames noind).
+Proof.
+  unfold typed_trans, TaskGen.typed_trans.
+  intros tsk Hty tr [Htr | []]; subst.
+  constructor.
+  - rewrite fold_all_ctx_gamma_eq. simpl_task.
+    admit.
+  - rewrite fold_all_ctx_gamma_eq, fold_all_ctx_delta_eq. simpl_task.
+    rewrite map_snd_combine by solve_len.
+    rewrite map_map.
+    rewrite Forall_map, Forall_forall.
+    intros [n f] Hin. simpl.
+    unfold rewriteF'.
+    Print rewriteF'.
+
+
+    2: rewrite !map_length.
+
+
+
+  
+  
+  
+   Search task_gamma fold_all_ctx.
+  
+   simpl.
+  Print task_typed.
+
+
+  unfold fold_comp. simpl.
+
+
+  unfold task_valid, TaskGen.task_valid in *.
+  split; auto.
+  intros gamma_valid Hty'.
+  (*Temp*) Opaque fold_all_ctx.
+  unfold fold_comp in Hallval.
+  (*Use gamma, delta, goal lemmas*)
+  
+  
+   simpl.
+  Print typed_trans.
